\subsection{a} Derive the MLE for $\mu$ and its distribution for a fixed set of sampling increments $\{h_i\}:\sum_{i=1}^nh_i=T$.

\begin{solution} Finding estimate for $\mu$.

The Likelihood function for MLE for $\mu$:

\begin{equation}
\begin{aligned}
\mathcal{L}\left(\mu,\sigma^2|Y_1, Y_2, \ldots, Y_n\right) & = Pr(Y_1, Y_2, \ldots, Y_n|\mu, \sigma^2) \\
																										& = \prod_{i=1}^n\frac{1}{\sqrt{2\pi\sigma^2h_i}}\exp\left(\frac{-(Y_i-\mu h_i)^2}{2\sigma^2h_i}\right)
\end{aligned}
\end{equation}

And the log-likelihood function:
\begin{equation}
\label{e:loglikelihood2a}
\begin{aligned}
\mathit{l}\left(\mu,\sigma^2|Y_1, Y_2, \ldots, Y_n\right) & = \sum_{i=1}^n\ln\left(\frac{1}{\sqrt{2\pi\sigma^2h_i}}\right) + \sum_{i=1}^n\left(\frac{-(Y_i-\mu h_i)^2}{2\sigma^2h_i}\right)
\end{aligned}
\end{equation}

To find maximum of log-likelihood function we take derivative with respect to $\mu$:

\begin{equation}
\begin{aligned}
\frac{\partial}{\partial\mu}\mathit{l}\left(\mu,\sigma|Y_1, Y_2, \ldots, Y_n\right) 
								 = \sum_{i=1}^n\frac{2h_i(Y_i-\mu h_i)}{2\sigma^2h_i}
								 = \sum_{i=1}^n\frac{(Y_i-\mu h_i)}{\sigma^2}
\end{aligned}
\end{equation}

Log-likelihood function will be maximized when $\frac{\partial}{\partial\mu}\mathit{l}\left(\mu,\sigma|Y_1, Y_2, \ldots, Y_n\right) = 0$:

\begin{equation}
\sum_{i=1}^n\frac{(Y_i-\mu h_i)}{\sigma^2} = 0 \Longrightarrow
								 \sum_{i=1}^n(Y_i-\mu h_i) = 0 \Longrightarrow
								 \sum_{i=1}^nY_i = \mu\sum_{i=1} h_i
\end{equation}

\begin{equation}
\hat{\mu} = \frac{1}{T}\sum_{i=1}^nY_i
\end{equation}

\end{solution}

\begin{solution} Finding distribution for $\hat{\mu}$.

Since $Y_i \thicksim \mathbi{N}\left(\mu h_i, \sigma^2 h_i\right)$ the Moment Generating Function of $Y_i$ will be:

\begin{equation}
\mathbi{M}_{Y_i}(t) = \exp\left(\mu h_it + \frac{\sigma^2 h_i t^2}{2}\right);
\end{equation}

The moment generating function of sum of r.v's is equal to product of their MGF's :

\begin{equation}
\begin{aligned}
\mathbi{M}_{Z}(t) & = \prod_{i=1}^{n}\exp\left(\mu h_it + \frac{\sigma^2 h_i t^2}{2}\right) 
									  = \exp\left(\mu t \sum_{i=1}^{n}h_i + \frac{\sigma^2t^2 \sum_{i=1}^{n}h_i}{2}\right) \\
									& = \exp\left(\mu Tt + \frac{\sigma^2Tt^2}{2}\right)
\end{aligned}
\end{equation}

where $Z=\sum_{i=1}^{n}Y_i$.


The $\mathbi{M}_{Z}(t)$ is a MGF of Normal distribution therefore:
 
\begin{equation}
\begin{aligned}
\hat{\mu} = \frac{1}{T}Z & \thicksim \mathbi{N}\left(\mu, \frac{\sigma^2}{T}\right)\square
\end{aligned}
\end{equation}

\end{solution}